NewTranslate/The_Laws.thy
@@ -2,13 +2,32 @@ theory The_Laws
   imports 
     "./Predicates"
     "../Programming/IntroPar_Big"
-
+    "../Programming/State_Relations"
+    "../Programming/Assignments"
 begin
 
 text \<open>Below are some results around program refinement\<close>
 
-locale laws = strong_spec + intro_par_big
+locale laws = strong_spec + intro_par_big + state_relations + expressions + assignments
 begin
+
+lemma relat_ge: "\<lceil>\<lpred>q1\<rpred> \<sqinter> \<lpred>q2\<rpred>\<rceil> \<ge> \<lparr>\<lpred>q1 |\<and>| q2\<rpred>\<rparr>"
+ by (metis (mono_tags, opaque_lifting) Int_subset_iff conj.sync_mono conj_chaos lambda_and_def pspec_strengthen rel_eq spec_def term_nonaborting)
+
+lemma relat_le "\<lparr>\<lpred>q1 |\<and>| q2\<rpred>\<rparr> \<ge> \<lceil>\<lpred>q1\<rpred> \<sqinter> \<lpred>q2\<rpred>\<rceil>"
+proof -
+  have "\<lparr>\<lpred>q1 |\<and>| q2\<rpred>\<rparr> = \<lparr>\<lpred>(\<lambda>s. q1 s \<and> q2 s)\<rpred>\<rparr>"
+    by (simp add: lambda_and_def) 
+  have "... = \<lparr>{s. q1 s \<and> q2 s}\<rparr>"
+    by (simp add: relation_def)
+  have "... = \<lparr>{s. q1 s} \<inter> {s. q2 s}\<rparr>"
+    by (simp add: Collect_conj_eq)
+  have "... = \<lparr>\<lpred>q1\<rpred> \<inter> \<lpred>q2\<rpred>\<rparr>"
+    by (simp add: relation_def)
+  have "... = \<lparr>\<lpred>q1\<rpred> \<sqinter> \<lpred>q2\<rpred>\<rparr>"
+    by auto
+  have "... \<ge> \<lceil>\<lpred>q1\<rpred> \<sqinter> \<lpred>q2\<rpred>\<rceil> \<iinter> term" by sledgehammer
+qed
 
 lemma monotonicity:
   assumes "c0 \<ge> c1 \<and> d0 \<ge> d1"
@@ -35,8 +54,8 @@ lemma strengthen_post_pre:
   by (metis assms dom_restrict prod.collapse spec_strengthen_under_pre)
 
 lemma sequential:
-  shows "\<lparr>\<lpred>q1\<rpred> O \<lpred>q2\<rpred>\<rparr> \<ge> \<lparr>\<lpred>q1\<rpred>\<triangleright>\<lrel>p1\<rrel>\<rparr>;\<lbrace>\<lrel>p1\<rrel>\<rbrace>;\<lparr>\<lpred>q2\<rpred>\<rparr>"
-  using spec_seq_introduce by auto
+  shows "\<lparr>\<lpred>q1 \<Zcomp> q2\<rpred>\<rparr> \<ge> \<lparr>\<lpred>q1\<rpred>\<triangleright>\<lrel>p1\<rrel>\<rparr>;\<lbrace>\<lrel>p1\<rrel>\<rbrace>;\<lparr>\<lpred>q2\<rpred>\<rparr>"
+  by (simp add: relseqeq spec_seq_introduce)
 
 lemma weaken_rely:
   assumes "\<forall> s. r1 s \<longrightarrow> r2 s"
@@ -62,8 +81,8 @@ lemma introduce_guar:
   using guar_introduce by force
 
 lemma merge_guars:
-  shows "(guar \<lpred>g1\<rpred>) \<iinter> (guar \<lpred>g2\<rpred>) \<ge> guar \<lpred>(\<lambda>s. g1 s \<and> g2 s)\<rpred>"
-  using conj_refine strengthen_guar by presburger
+  shows "(guar \<lpred>g1\<rpred>) \<iinter> (guar \<lpred>g2\<rpred>) \<ge> guar \<lpred>(g1 |\<and>| g2)\<rpred>"
+  by (metis conj_refine lambda_and_def strengthen_guar)
 
 lemma distrib_guar_seq:
   shows "(guar g) \<iinter> (c;d) \<ge> ((guar g) \<iinter> c) ; ((guar g) \<iinter> d)"
@@ -73,15 +92,105 @@ lemma distrib_guar_par:
   shows "(guar g) \<iinter> (c\<parallel>d) \<ge> ((guar g) \<iinter> c) \<parallel> ((guar g) \<iinter> d)"
   using guar_distrib_par by blast
 
-(*
 lemma distrib_guar_multipar:
-  shows "(guar g) \<iinter> (\<parallel>i ci) \<ge> \<parallel>i ((guar g) \<iinter> ci)"
-  by sledgehammer
-*)
+  assumes "finite A"
+  assumes "A \<noteq> {}"
+  shows "((guar g) \<iinter> (\<parallel>\<parallel>\<in>A. (\<lambda>x. x))) \<ge> (\<parallel>\<parallel>\<in>A. (\<lambda>x. (guar g) \<iinter> x))"
+  by (smt (verit, del_insts) assms(1) assms(2) conj_setpar_distrib guar_distrib_seq guar_par_idem guar_seq_idem local.conj.idem setpar.cong)
 
 lemma restrict_frame:
-  assumes "X \<subseteq> Y"
-  shows "X:c \<ge> Y:c"
+  assumes "Y |\<subseteq>| X"
+  shows "X:\<^sub>sc \<ge> Y:\<^sub>sc"
+  using assms conj.sync_mono_left guar_strengthen id_bar_narrow var_frame_set_def by presburger
+
+lemma introduce_para:
+  shows "(rely \<lpred>r\<rpred>) \<iinter> \<lparr>\<lpred>(q1 |\<and>| q2)\<rpred>\<rparr> \<ge> 
+         ((rely \<lpred>(r |\<or>| r1)\<rpred>) \<iinter> (guar \<lpred>r2\<rpred>) \<iinter> \<lparr>\<lpred>q1\<rpred>\<rparr>)
+         \<parallel> ((rely \<lpred>(r |\<or>| r2)\<rpred>) \<iinter> (guar \<lpred>r1\<rpred>) \<iinter> \<lparr>\<lpred>q2\<rpred>\<rparr>)"
+proof - 
+  have "(rely \<lpred>r\<rpred>) \<iinter> \<lparr>\<lpred>(q1 |\<and>| q2)\<rpred>\<rparr> \<ge> (rely \<lpred>r\<rpred>) \<iinter> \<lparr>\<lpred>(q1 |\<and>| q2)\<rpred>\<rparr> \<iinter> term" 
+    using conj_conjoin_non_aborting term_nonaborting by force
+  also have "(rely \<lpred>r\<rpred>) \<iinter> \<lceil>\<lpred>q1\<rpred> \<sqinter> \<lpred>q2\<rpred>\<rceil> \<iinter> term \<ge> (rely \<lpred>r\<rpred>) \<iinter> \<lparr>\<lpred>(q1 |\<and>| q2)\<rpred>\<rparr> \<iinter> term" (is "_ \<ge> ?rhs")
+    using conj.sync_mono_right local.conj_commute relat_eq by presburger
+  also have  \<ge> ((guar \<lpred>r |\<or>| r2\<rpred>) \<iinter> (rely \<lpred>r |\<or>| r1\<rpred>) \<iinter> \<lparr>\<lpred>q1\<rpred>\<rparr> \<parallel> (guar \<lpred>r |\<or>| r1\<rpred>) \<iinter> (rely \<lpred>r |\<or>| r2\<rpred>) \<iinter> \<lparr>\<lpred>q2\<rpred>\<rparr>) \<iinter> term" by sledgehammer
+qed
+
+lemma introduce_multi_para:
+  assumes "finite A"
+  assumes "A \<noteq> {}"
+  shows "(rely \<lpred>r\<rpred>) \<iinter> \<lparr>\<lpred>|\<And>|A\<rpred>\<rparr> \<ge> (\<parallel>\<parallel>\<in>A. (\<lambda>q. (guar \<lpred>r1\<rpred>) \<iinter> (rely \<lpred>(r |\<or>| r1)\<rpred>) \<iinter> \<lparr>\<lpred>q\<rpred>\<rparr>))" 
+  sorry
+
+lemma trading:
+  shows "(rely \<lpred>r\<rpred>) \<iinter> (guar \<lpred>g\<rpred>) \<iinter> \<lparr>\<lpred>q\<rpred>\<rparr> = (rely \<lpred>r\<rpred>) \<iinter> (guar \<lpred>g\<rpred>) \<iinter> \<lparr>\<lpred>(r |\<or>| g)\<rpred>\<^sup>* \<inter> \<lpred>q\<rpred>\<rparr>"
+  sorry
+
+definition pstable :: "('state \<Rightarrow> bool) \<Rightarrow> (('state*'state) \<Rightarrow> bool) \<Rightarrow> bool"
+  where "pstable p r \<equiv> \<forall> s. r s \<longrightarrow> (p (fst s) \<longrightarrow> p (snd s))"
+
+definition qtolerates :: "('state \<Rightarrow> bool) \<Rightarrow> (('state*'state) \<Rightarrow> bool) \<Rightarrow> (('state*'state) \<Rightarrow> bool) \<Rightarrow> bool" 
+  where "qtolerates p q r
+     \<equiv> (pstable p r)
+     \<and> (\<forall>s. (p (fst s) \<and> (r \<Zcomp> q) s) \<longrightarrow> q s)
+     \<and> (\<forall>s. (p (fst s) \<and> (q \<Zcomp> r) s) \<longrightarrow> q s)"
+
+definition const_exp :: "('state, 'v) expr \<Rightarrow> (('state*'state) \<Rightarrow> bool) \<Rightarrow> bool"
+  where "const_exp e r \<equiv> \<forall> (s, s')\<in>\<lpred>r\<rpred>. eval e s = eval e s'"
+
+fun sin_ref_exp :: "('state,'v) expr \<Rightarrow> (('state*'state) \<Rightarrow> bool) \<Rightarrow> bool" where
+  "sin_ref_exp (Constant k) r = True" | 
+  "sin_ref_exp (Variable accessor) r = True" | 
+  "sin_ref_exp (UnaryOp oper e1) r = (sin_ref_exp e1 r)" |
+  "sin_ref_exp (BinaryOp oper e1 e2) r = 
+      ((sin_ref_exp e1 r) \<and> (sin_ref_exp e2 r) \<and> 
+      ((const_exp e1 r) \<or> (const_exp e2 r)))"
+
+definition atomic_exp :: "('b \<Rightarrow> bool) \<Rightarrow> ('b*'b \<Rightarrow> bool) \<Rightarrow> 'a" ("\<langle>_,_\<rangle>" [30, 30])
+  where "atomic_exp p q \<equiv> opt (\<lrel>p\<rrel> \<triangleleft> \<lpred>q\<rpred>)"
+
+lemma intro_atomic:
+  assumes "pstable p r \<and> refl \<lpred>g\<rpred> \<and> qtolerates p q r"
+  shows "(guar \<lpred>g\<rpred>) \<iinter> (rely \<lpred>r\<rpred>) \<iinter> \<lbrace>\<lrel>p\<rrel>\<rbrace>;\<lparr>\<lpred>q\<rpred>\<rparr> \<ge> (rely \<lpred>r\<rpred>) \<iinter> \<langle>p, (g |\<and>| q)\<rangle>"
+  sorry
+
+lemma local_ass:
+  assumes "sin_ref_exp e r"
+  assumes "const_exp e r"
+  assumes "pstable p r"
+  assumes "qtolerates p q r"
+  assumes "refl \<lpred>g\<rpred>"
+  assumes "\<forall>s. (p (fst s) \<and> id\<^sub>x s) \<longrightarrow> (g |\<and>| q) (fst s, set_var x (eval e (fst s)) (snd s))"
+  shows "(rely \<lpred>r\<rpred> ) \<iinter> (guar \<lpred>g\<rpred>) \<iinter> \<lbrace>\<lrel>p\<rrel>\<rbrace>;x:\<^sub>f\<lparr>\<lpred>q\<rpred>\<rparr> \<ge> x ::= e"
+  sorry
+
+lemma post_ass:
+  assumes "sin_ref_exp e r"
+  assumes "const esp e r"
+  assumes "pstable p0 r"
+  assumes "pstable p1 r"
+  assumes "qtolerates p q r"
+  assumes "refl \<lpred>g\<rpred>"
+  assumes "\<forall>s. (p1 (fst s) \<and> id\<^sub>x s) \<longrightarrow> g (fst s, set_var x (eval e (fst s)) (snd s))"
+  shows "(rely \<lpred>r\<rpred>) \<iinter> (guar \<lpred>g\<rpred>) \<iinter> \<lbrace>\<lrel>p0\<rrel>\<rbrace>;x:\<^sub>f\<lparr>\<lpred>q\<rpred>\<rparr> \<ge> ((rely \<lpred>r\<rpred>) \<iinter> (guar \<lpred>g\<rpred>) \<iinter> \<lbrace>\<lrel>p0\<rrel>\<rbrace>;\<lparr>\<lpred>(\<lambda>(s, s').q (s, set_var x (eval e s') s') \<and> p1 s')\<rpred>\<rparr>);(x ::= e)"
+  sorry
+
+lemma rely_ass:
+  fixes gte :: "'d \<Rightarrow> 'd \<Rightarrow> bool" (infix "\<succeq>" 50)
+  assumes "pstable p r"
+  assumes "const_exp (Constant x) r"
+  assumes "sin_ref_exp e r"
+  assumes "refl \<lpred>case_prod gte\<rpred> \<and> trans \<lpred>case_prod gte\<rpred>"
+  assumes "\<forall>s. ((id\<^sub>x s \<or> r s) \<longrightarrow> ((eval e (fst s)) \<succeq> (eval e (snd s)))) \<and> (((p (fst s) \<and> id\<^sub>x s)) \<longrightarrow> g (fst s, set_var x (eval e (fst s)) (snd s)))"
+  shows "(rely \<lpred>r\<rpred>) \<iinter> (guar \<lpred>g\<rpred>) \<iinter> \<lbrace>\<lrel>p\<rrel>\<rbrace>;x:\<^sub>f\<lparr>\<lpred>(\<lambda>(\<sigma>, \<sigma>'). eval e \<sigma> \<succeq> get_var x \<sigma>' \<and> get_var x \<sigma>' \<succeq> eval e \<sigma>')\<rpred>\<rparr> \<ge> (x ::= e) "
+  sorry
+
+lemma intro_var:
+  assumes "pstable p r"
+  assumes "qtolerates p q r"
+  shows "(rely \<lpred>r\<rpred>) \<iinter> (guar \<lpred>(\<lambda>(s, s'). get_var x s' = get_var x s \<and> (\<exists>s. g s))\<rpred>) \<iinter> \<lbrace>\<lrel>p\<rrel>\<rbrace>;Y:\<^sub>s\<lparr>\<lpred>(\<lambda>s. \<exists>s. q s)\<rpred>\<rparr> \<ge> 
+         (rely \<lpred>(\<lambda>(s, s'). get_var x s' = get_var x s \<and> (\<exists>s. r s))\<rpred>) \<iinter> (guar \<lpred>g\<rpred>) \<iinter> \<lbrace>\<lrel>(\<lambda>s. \<exists>s. p s)\<rrel>\<rbrace>;({|x|} |\<union>| Y):\<^sub>s\<lparr>\<lpred>q\<rpred>\<rparr>" 
+  sorry (*this one is written wrong with the \<exists>*)
+
 
 end
 
